TypeTheorems.thy
@@ -1,145 +1,6 @@
-theory gASPFuturesTypeSystem imports gASPFutures begin
+theory TypeTheorems imports gASPFuturesTypeSystem begin
 
-definition BuildTypeEnv ::"(ASPType * VarName) list \<Rightarrow> VarName \<Rightarrow>ASPType option"
-where
-"BuildTypeEnv VarDeclList =  (map_of (map prod.swap (VarDeclList)))"
-
-inductive Subtype :: "Program\<Rightarrow>ASPType \<Rightarrow>ASPType \<Rightarrow>bool "  (" _\<turnstile>_\<sqsubseteq>_" 50)
- where
- "P\<turnstile>T\<sqsubseteq>T"
-|
- "P\<turnstile>BType T\<sqsubseteq>FutType T"
-|
- "P\<turnstile>BType (TObj C)\<sqsubseteq>BType AnyObject"
-|
- "P\<turnstile>FutType (TObj C)\<sqsubseteq>FutType AnyObject"
-
-inductive TypeValue :: "Program\<Rightarrow>Configuration\<Rightarrow>Value \<Rightarrow> ASPType \<Rightarrow> bool"  ("_,_\<turnstile>\<^sub>V_:_" 50)
-where
- "P,Conf \<turnstile>\<^sub>V ASPInt n: BType Integer"
-|
- "P,Conf \<turnstile>\<^sub>V ASPBool b: BType Boolean"
-|
- "P,Conf \<turnstile>\<^sub>V null :  BType (AnyObject)"
-|
- "Acts \<alpha>= Some(AO C' state R Ec Rq)
-\<Longrightarrow> P,Cn Acts Futs \<turnstile>\<^sub>V ActRef \<alpha>:  BType (TObj C')"  (*dynamic obj*)
-|
- "Futs f = Some(T,V)
-\<Longrightarrow> P,Cn Acts Futs \<turnstile>\<^sub>V FutRef f: FutType T"  (*dynamic fut*)
-
-inductive TypeExpression :: "Program\<Rightarrow>Configuration\<Rightarrow> (VarName \<rightharpoonup>ASPType)\<Rightarrow> ClassName\<Rightarrow>Expression \<Rightarrow>ASPType \<Rightarrow> bool"  ("_,_,_ in _\<turnstile>\<^sub>E_:_" 50)
- where
- " P,Config \<turnstile>\<^sub>V v:T \<Longrightarrow> P,config,\<Gamma> in C \<turnstile>\<^sub>E Val v:T"
-|
-" P,Cn Acts Futs,\<Gamma> in C \<turnstile>\<^sub>E Var This:  BType (TObj C)  (*This*)
-  " 
-|
-" \<Gamma> x = Some T \<Longrightarrow>P,Cn Acts Futs,\<Gamma>  in C\<turnstile>\<^sub>E Var (Id x) : T (* Var or field reference *)
-  "
-|
-"\<lbrakk> P,Config,\<Gamma> in C \<turnstile>\<^sub>E e:BType Integer; P,Config,\<Gamma> in C \<turnstile>\<^sub>E e':BType Integer
-\<rbrakk> \<Longrightarrow>
-P,Config,\<Gamma> in C \<turnstile>\<^sub>Ee+\<^sub>Ae':BType Integer"
-|
-"P\<turnstile>T\<sqsubseteq>T' \<Longrightarrow>  P,Config,\<Gamma> in C \<turnstile>\<^sub>E e:T \<Longrightarrow> P,Config,\<Gamma> in C \<turnstile>\<^sub>E e:T' " (* subtype*)
-
-
-inductive TypeRhs  :: "Program\<Rightarrow>Configuration\<Rightarrow> (VarName \<rightharpoonup>ASPType)\<Rightarrow> ClassName\<Rightarrow> Rhs \<Rightarrow>ASPType \<Rightarrow> bool"  ("_,_,_ in _\<turnstile>\<^sub>R_:_" 50)
- where
-  (* Expression *)
- " P,Config,\<Gamma> in C \<turnstile>\<^sub>E e:T \<Longrightarrow> P,Config,\<Gamma> in C \<turnstile>\<^sub>R (Expr e):T"
-|  (* method call*)
- "\<lbrakk> P,Config,\<Gamma> in C \<turnstile>\<^sub>E e:BType (TObj C') ; fetchClass P C' = Some Class;
-   fetchMethodInClass Class m = Some Meth;
-   param_types= map fst (MParams Meth) ; length param_types = length el ; \<forall> i<length el. (P,Config,\<Gamma> in C \<turnstile>\<^sub>E el!i:(param_types!i)) \<rbrakk>
-\<Longrightarrow> P,Config,\<Gamma> in C \<turnstile>\<^sub>R (e.\<^sub>Am(el)):MakeFutureType (MRType Meth)"
-|  (* new active *)
-"\<lbrakk>  fetchClass P C' = Some Class;
-   Class_param_types = map fst (ClassParameters Class);
-   length Class_param_types = length el ; \<forall> i<length el. (P,Config,\<Gamma> in C \<turnstile>\<^sub>E el!i:(Class_param_types!i)) \<rbrakk>
-\<Longrightarrow> P,Config,\<Gamma> in C \<turnstile>\<^sub>R (newActive C'(el)):BType (TObj C')"
-| (* Get *)
-" P,Config,\<Gamma> in C \<turnstile>\<^sub>E e:(FutType T)    \<Longrightarrow> P,Config,\<Gamma> in C \<turnstile>\<^sub>R (Get e):BType (T)"
-|
-"P\<turnstile>T\<sqsubseteq>T' \<Longrightarrow>  P,Config,\<Gamma> in C \<turnstile>\<^sub>R e:T \<Longrightarrow> P,Config,\<Gamma> in C \<turnstile>\<^sub>R e:T' "   (* subtype*)
-
-inductive TypeStatement  :: "Program\<Rightarrow>Configuration\<Rightarrow> (VarName \<rightharpoonup>ASPType)\<Rightarrow> ClassName\<Rightarrow>Statement\<Rightarrow> bool"  ("_,_,_ in _\<turnstile>\<^sub>S _ " 50)
-and TypeStatementList ::"Program\<Rightarrow>Configuration\<Rightarrow> (VarName \<rightharpoonup>ASPType)\<Rightarrow> ClassName\<Rightarrow>Statement list\<Rightarrow> bool"  ("_,_,_ in _\<turnstile>\<^sub>L _ " 50)
- where
- "\<lbrakk> P,Config,\<Gamma> in C \<turnstile>\<^sub>R a:T; 
-    \<Gamma> x = Some T' ; P\<turnstile>T\<sqsubseteq>T'
-\<rbrakk> \<Longrightarrow>
-P,Config,\<Gamma> in C \<turnstile>\<^sub>S (x=\<^sub>A a) "
-|
- "\<lbrakk> fetchClass P C = Some Class;
-   fetchMethodInClass Class m = Some Meth;
-   MRType Meth = T';
-   P,Config,\<Gamma> in C \<turnstile>\<^sub>E e:T; 
-    \<Gamma> x = Some T' ; P\<turnstile>T\<sqsubseteq>T'
-\<rbrakk> \<Longrightarrow>
-P,Config,\<Gamma> in C \<turnstile>\<^sub>S return e "
-|
- "\<lbrakk>
-   P,Config,\<Gamma> in C \<turnstile>\<^sub>E e:BType Boolean; 
-   P,Config,\<Gamma> in C \<turnstile>\<^sub>L sl;  P,Config,\<Gamma> in C \<turnstile>\<^sub>L sl'
-\<rbrakk> \<Longrightarrow>
-P,Config,\<Gamma> in C \<turnstile>\<^sub>S IF e THEN sl ELSE sl' "
-|
-"P,Config,\<Gamma> in C \<turnstile>\<^sub>L [] "
-|
-"P,Config,\<Gamma> in C \<turnstile>\<^sub>S s\<Longrightarrow> P,Config,\<Gamma> in C \<turnstile>\<^sub>L sl\<Longrightarrow>P,Config,\<Gamma> in C \<turnstile>\<^sub>L s;;sl "
-
-
-fun TypeClass :: "Program \<Rightarrow> Class \<Rightarrow>bool" ("_ \<turnstile>\<^sub>C _ " 50)
-where
-" (P\<turnstile>\<^sub>CClass) = (let C_param_env = (map_of (map prod.swap (ClassParameters Class))) in
-               (\<forall> M\<in> set (Methods Class). 
-               let \<Gamma> = C_param_env ++ (map_of (map prod.swap (LocalVariables M))) ++ (map_of (map prod.swap (MParams M))) in
-               (P,EmptyConfig,\<Gamma> in (Name Class) \<turnstile>\<^sub>L (Body M) ) ) ) "
-
-primrec TypeProgram :: "Program \<Rightarrow>bool" ("\<turnstile>\<^sub>P _ " 50)
-where
-" (\<turnstile>\<^sub>PProg CL MainVars MainBody) = (let P = Prog ((MainObjClass MainVars)#CL) MainVars MainBody in
-                          ( (\<forall> C\<in>set CL. (P\<turnstile>\<^sub>CC)) \<and>
-                            (let \<Gamma> = (map_of (map prod.swap (MainVars))) in
-                              (P,EmptyConfig,\<Gamma> in (''MainClass'') \<turnstile>\<^sub>L MainBody )  ) ) )
-"
-
-inductive TypeRequest :: "Program \<Rightarrow> Configuration\<Rightarrow> ClassName \<Rightarrow>Request \<Rightarrow> bool"  ("_,_ in _ \<turnstile>\<^sub>Q _" 50)
-where 
-" \<lbrakk> fetchClass P C =   Some Class ;
-    fetchMethodInClass Class m = Some Meth; 
-    param_types= map fst (MParams Meth);
-    length vl = length param_types ;  \<forall> i <length vl . (P, Cn Acts Futs\<turnstile>\<^sub>V(vl!i):(param_types!i));
-    Futs f = Some (T, Undefined); T=GetBasicType (MRType Meth)
-\<rbrakk>
-\<Longrightarrow>P,Cn Acts Fut in C\<turnstile>\<^sub>Q(f,m,vl)"
-
-primrec TypeConfig :: "Program \<Rightarrow>Configuration \<Rightarrow>bool" ("_ \<turnstile> _ " 50)
-where
-" (P\<turnstile>Cn AOs Futures) =
-((\<forall> Act\<in> ran AOs. case Act of (AO C state R Ec Rq) \<Rightarrow>
-   (\<exists> CL . (fetchClass P C = Some CL \<and>
-    (
-     (* check state *)
-     ( (  \<forall> x v. (state(x) =Some  v \<longrightarrow> (\<exists> T . (T,x)\<in> set (ClassParameters CL) \<and> (P,Cn AOs Futures\<turnstile>\<^sub>V v: T))) ) )
-     (* check request queue*)
-     \<and> (\<forall> R'\<in>set Rq. (P, (Cn AOs Futures) in C \<turnstile>\<^sub>Q R' ) )
-     (* check current request*)
-     \<and> 
-     (case R of Some  (f,m,vl) \<Rightarrow>
-         (\<exists> Meth. fetchMethodInClass CL m = Some Meth \<and>
-           (P, Cn AOs Futures in C \<turnstile>\<^sub>Q (f,m,vl)) 
-           \<and> (case Ec of (locs,Stl) \<Rightarrow> ( \<forall> s\<in>set Stl. 
-             (P,Cn AOs Futures,(BuildTypeEnv (ClassParameters CL))++(BuildTypeEnv (LocalVariables Meth))++(BuildTypeEnv (MParams Meth)) in C \<turnstile>\<^sub>S s)
-        )) ) ) )))) \<and>
-   (* Futures *)
-(\<forall> futs\<in> ran Futures. case futs of
-      (T,Undefined) \<Rightarrow> True |
-      (T,FutVal v) \<Rightarrow> (P,Cn AOs Futures \<turnstile>\<^sub>V v: (FutType T))))
-"
-
+section{* Basic Lemmas *}
 
 lemma TypeStatementList_TypeStatement[rule_format]: 
 "(P,Config,\<Gamma> in C \<turnstile>\<^sub>L Stl)  \<longrightarrow> (S \<in> set Stl\<longrightarrow> (P,Config,\<Gamma> in C \<turnstile>\<^sub>S S))"
@@ -232,8 +93,9 @@ lemma TypeStatementList_extendconfiguration_AO:
 " (P,Cn AOs futs,\<Gamma> in C \<turnstile>\<^sub>L Stl) \<Longrightarrow> \<alpha>\<notin>(dom AOs) \<Longrightarrow>f\<notin> dom futs \<Longrightarrow> (P, Cn (AOs(\<alpha>\<mapsto>X)) (futs(f\<mapsto>Y)),\<Gamma> in C \<turnstile>\<^sub>L Stl) "
 by (case_tac Y,insert TypeStatement_extendconfiguration_AO_Pre,auto)
 
+section{* Well-typed initial configuraiton *}
 
-lemma WTinitialconfiguration: "\<turnstile>\<^sub>P Prog  CL Vars Stl \<Longrightarrow> Prog  ((MainObjClass Vars)#CL) Vars Stl \<turnstile> InitialConfiguration (Prog  CL Vars Stl)"
+theorem WTinitialconfiguration: "\<turnstile>\<^sub>P Prog  CL Vars Stl \<Longrightarrow> Prog  ((MainObjClass Vars)#CL) Vars Stl \<turnstile> InitialConfiguration (Prog  CL Vars Stl)"
 apply (unfold InitialConfiguration_def BuildInitialConfigurationfromVarsStl_def)
 apply (auto,unfold Let_def fetchClass_def fetchMethodInClass_def MainObjClass_def MainMethodEmptyBody_def,auto)
 apply (intro gASPFuturesTypeSystem.TypeRequest.intros, auto simp: fetchClass_def fetchMethodInClass_def )
